% !TeX root = document.tex
% !TeX encoding = UTF-8 Unicode

\section{Observer Design}%
\label{sec:observer-design}

\subsection{Bank of Observers}%
\label{subsec:bank-of-observers}

\begin{slide}{Bank of Observers}
  \input{imgs/schematic}
\end{slide}

\subsection{Observer Design}%
\label{subsec:observer-design}

\begin{slide}{Observer Design}
  \begin{columns}[c]
    \begin{column}{0.55\textwidth}
      \begin{equation}
        \begin{aligned}
          \textrm{arg min } & \norm{P}_{2}    \\
          \textrm{s.t. }    & \dot{V} \prec 0 \\
                            & P \succ 0,
        \end{aligned}
      \end{equation}
      %
      where
      %
      \begin{align}
        \dot{V} \equiv & \begin{bmatrix}
                           X        & W  \\
                           W^{\top} & -I
                         \end{bmatrix},                                         \\
        \lambda\in     & \mathbb{R}^{+} \textrm{ is a free constant}, \nonumber \\
        P              & \textrm{ is a semidefinite positve matrix} \nonumber
      \end{align}
      %
      with
      %
      \begin{align}
        \begin{split}
          X = & \hat{A}^{\top}F^{\top}P - \hat{A}^{\top}C^{\top}\hat{E}^{\top} -                 \\
          & \hat{C}^{\top}\hat{K}^{\top} + PF\hat{A} - \hat{E}C\hat{A} - \hat{K}\hat{C} - \lambda{}I,
        \end{split} \\
        W = & \sqrt{\lambda}(PF - \hat{E}C).
      \end{align}
    \end{column}%
    \hfill%
    \begin{column}{0.55\textwidth}
      \begin{align}
        \begin{split}
          \hat{A} & = AF^{+},              \\
          \hat{C} & = CF^{+},              \\
          \hat{E} & = PE = PU + \hat{Y}V,  \\
          \hat{K} & = PK,                  \\
          \hat{Y} & = PY.
        \end{split} \\\nonumber\\
        \begin{split}
          K & = P^{-1}\hat{K},  \\
          Y & = P^{-1}\hat{Y},  \\
          E & = U + YV,         \\
          R & = F - EC,         \\
          N & = (RA - KC)F^{+}, \\
          J & = K + NE,         \\
          H & = RB.
        \end{split}
      \end{align}
    \end{column}%
  \end{columns}
\end{slide}

\begin{slide}{Observer Design Development}
  \begin{columns}[c]
    \begin{column}{0.55\textwidth}
      \begin{align}
        \begin{split}
          e & = \hat{z} - z   \\
          & = w + Ey - Fx   \\
          & = w + ECx - Fx.
        \end{split} \\
        \begin{split}
          \dot{e} & = \dot{w} + (EC-F)\dot{x}              \\
          & = Nw + Jy + Hu + (EC-F)(Ax + Bu + Lf)  \\
          & = Ne + (NF-NEC+ECA-FA+JC)x +           \\
          & \phantom{=~} (H+ECB-FB)u + (ECL-FL)f.
        \end{split}
      \end{align}
    \end{column}%
    \hfill%
    \begin{column}{0.55\textwidth}
      \begin{align}
        \begin{split}
          N \textrm{ must be Hurwitz-stable}, &      \\
          N(F-EC)-(F-EC)A+JC                  & = 0, \\
          H-(F-EC)B                           & = 0.
        \end{split} \\\nonumber\\
        \begin{split}
          (F-EC)L_{i} & = 0,     \\
          (F-EC)L_{n} & \neq 0.
        \end{split}
      \end{align}
    \end{column}%
  \end{columns}
\end{slide}

\begin{slide}{Observer Design Development}
  \begin{columns}[c]
    \begin{column}{0.55\textwidth}
      \begin{align}
        V             & = e^{\top}Pe,          \\
        \dot{e}       & = Ne-(F-EC)L_{n}f,     \\
        e             & \propto L_{n}f,        \\
        \norm{L_{n}f} & = \lambda{}\norm{e},   \\
        R             & = F-EC,                \\
        \dot{e}       & = Ne-R\lambda\norm{e}.
      \end{align}
    \end{column}%
    \hfill%
    \begin{column}{0.55\textwidth}
      \begin{align}
        \begin{split}
          \dot{V} & = \dot{e}^{\top}Pe + e^{\top}P\dot{e}                                     \\
          & = (Ne-\lambda{}R\norm{e})^{\top}Pe + e^{\top}P(Ne-\lambda{}R\norm{e})     \\
          & = e^{T}(N^{\top}P + PN)e - 2\lambda\norm{e^{\top}PR}\cdot\norm{e}         \\
          & \leq e^{T}(N^{\top}P + PN)e - \lambda(\norm{e^{\top}PR}^{2}+\norm{e}^{2}) \\
          & = e^{T}(N^{\top}P + PN - \lambda{}PRR^{\top}P - \lambda{}I)e.
        \end{split}
      \end{align}
    \end{column}%
  \end{columns}
\end{slide}

\begin{slide}{Observer Design Development}
  \begin{columns}[c]
    \begin{column}{0.55\textwidth}
      \begin{align}
        \begin{split}
          N(F-EC) & = RA-JC,                               \\
          NF      & = RA-(J-NE)C,                          \\
          K       & = J-NE,                                \\
          N       & = RAF^{+}-KCF^{+},
        \end{split} \\
        \begin{split}
          (F-EC)L_{i} & = 0,                                              \\
          ECL_{i}     & = FL_{i},                                         \\
          E           & = FL_{i}(CL_{i})^{+} + Y(I-(CL_{i})(CL_{i})^{+}), \\
          U           & = ECL_{i}L_{i}^{+},                               \\
          V           & = I-L_{i}L_{i}^{+},                               \\
          E           & = U+YV.
        \end{split}
      \end{align}
    \end{column}%
    \hfill%
    \begin{column}{0.55\textwidth}
      \begin{align}
        \begin{split}
          \dot{V} & = e^{T}((R\hat{A} - EC\hat{A} - K\hat{C})^{\top}P +                                         \\
          & P(R\hat{A} - EC\hat{A} - K\hat{C}) - \lambda{}PRR^{\top}P - \lambda{}I)e.                   \\
          & = \hat{A}^{\top}F^{\top}P - \hat{A}^{\top}C^{\top}\hat{E}^{\top} - \hat{C}^{\top}K^{\top} + \\
          & PF\hat{A} - \hat{E}C\hat{A} - K\hat{C} - \lambda{}PRR^{\top}P - \lambda{}I.
        \end{split}
      \end{align}
    \end{column}%
  \end{columns}
\end{slide}

\subsection{Residual Generator}%
\label{subsec:residual-generator}

\begin{slide}{Residual Generator}
  \begin{columns}[c]
    \begin{column}{0.55\textwidth}
      \begin{align}
        r(t) & = Gw(t) + My(t), \\
        \begin{split}
          M & = (C(1-L_{i}))^{\top},      \\
          G & = -M(I-CF^{+}E)^{-1}CF^{+},
        \end{split}
      \end{align}
    \end{column}%
    \hfill%
    \begin{column}{0.55\textwidth}
      \begin{align}
        \begin{split}
          r & = Gw + My                                     \\
            & = Q(y - Cx)                                   \\
            & = Q(y - CF^{-1}\hat{z})                       \\
            & = Q(y - CF^{-1}(w+Ey))                        \\
            & = Q((I-CF^{-1}E)y - CF^{-1}w),
        \end{split} \\
        \begin{split}
          M & = Q(I-CF^{-1}E),                              \\
          G & = -QCF^{-1}.
        \end{split}
      \end{align}
    \end{column}%
  \end{columns}
\end{slide}
